src/sys_verif/program_proof/demos/hashmap_proof.v
@@ -5,35 +5,45 @@
 |*)
 From sys_verif.program_proof Require Import prelude empty_ffi.
 
-From iris.base_logic.lib Require Import ghost_var.
 From New.proof Require Import sync.
 From New.generatedproof.sys_verif_code Require Import hashmap.
+From Perennial.algebra Require Import ghost_var.
 
 Module atomic_ptr.
 Section proof.
   Context `{hG: !heapGS Σ} `{!globalsGS Σ} {go_ctx: GoContext}.
+  Context `{!ghost_varG Σ loc}.
+
+  Implicit Types (γ: gname).
 
   #[global] Instance : IsPkgInit hashmap := define_is_pkg_init True%I.
   #[global] Instance : GetIsPkgInitWf hashmap := build_get_is_pkg_init_wf.
 
-  #[local] Definition lock_inv l (P: loc → iProp Σ): iProp _ :=
-    ∃ (mref: loc), "val" ∷ l ↦s[hashmap.atomicPtr :: "val"] mref ∗
-       "HP" ∷ P mref.
+  Definition own_ptr γ (x: loc) :=
+    ghost_var γ (DfracOwn (1/2)) x.
 
-  Definition is_atomic_ptr (l: loc) (P: loc → iProp Σ): iProp _ :=
-    ∃ (mu_l: loc),
-    "mu" ∷ l ↦s[hashmap.atomicPtr :: "mu"]□ mu_l ∗
-    "Hlock" ∷ is_Mutex mu_l (lock_inv l P).
-
-  #[global] Instance is_atomic_ptr_persistent l P : Persistent (is_atomic_ptr l P).
+  #[global] Instance own_ptr_timeless γ x : Timeless (own_ptr γ x).
   Proof. apply _. Qed.
 
-  Lemma wp_newAtomicPtr (P: loc → iProp Σ) (m_ref: loc) :
-    {{{ is_pkg_init hashmap ∗ P m_ref }}}
+  #[local] Definition lock_inv γ l : iProp _ :=
+    ∃ (mref: loc),
+      "val" ∷ l ↦s[hashmap.atomicPtr :: "val"] mref ∗
+      "Hauth" ∷ ghost_var γ (DfracOwn (1/2)) mref.
+
+  Definition is_atomic_ptr γ (l: loc) : iProp _ :=
+    ∃ (mu_l: loc),
+    "mu" ∷ l ↦s[hashmap.atomicPtr :: "mu"]□ mu_l ∗
+    "Hlock" ∷ is_Mutex mu_l (lock_inv γ l).
+
+  #[global] Instance is_atomic_ptr_persistent γ l : Persistent (is_atomic_ptr γ l).
+  Proof. apply _. Qed.
+
+  Lemma wp_newAtomicPtr (m_ref: loc) :
+    {{{ is_pkg_init hashmap }}}
       @! hashmap.newAtomicPtr #m_ref
-    {{{ (l: loc), RET #l; is_atomic_ptr l P }}}.
+    {{{ γ (l: loc), RET #l; is_atomic_ptr γ l ∗ own_ptr γ m_ref }}}.
   Proof.
-    wp_start as "HP".
+    wp_start as "_".
     wp_auto.
     wp_alloc mu_ptr as "mu".
     wp_auto.
@@ -42,54 +52,72 @@ Section proof.
     iNamed "Hptr".
     cbn [hashmap.atomicPtr.mu' hashmap.atomicPtr.val'].
     iPersist "Hmu".
-    iMod (init_Mutex (lock_inv l P)
-           with "mu [HP Hval]") as "Hlock".
+    iMod (ghost_var_alloc m_ref) as (γ) "[Hown Hauth]".
+    iMod (init_Mutex (lock_inv γ l)
+           with "mu [Hauth Hval]") as "Hlock".
     { iFrame. }
     wp_auto.
     wp_finish.
     iFrame "#∗".
   Qed.
 
-  Lemma wp_atomicPtr__load l (P: loc → iProp _) (Q: loc → iProp Σ) :
-    {{{ is_pkg_init hashmap ∗
-          is_atomic_ptr l P ∗ (∀ x, P x -∗ |={⊤}=> Q x ∗ P x) }}}
-      l @ (ptrT.id hashmap.atomicPtr.id) @ "load" #()
-    {{{ (x: loc), RET #x; Q x }}}.
+  Lemma wp_atomicPtr__load γ l :
+    ∀ (Φ: val → iProp Σ),
+    (is_pkg_init hashmap ∗
+    is_atomic_ptr γ l ∗
+    |={⊤,∅}=> ∃ x, own_ptr γ x ∗ (own_ptr γ x ={∅,⊤}=∗ Φ #x)) -∗
+    WP l @ (ptrT.id hashmap.atomicPtr.id) @ "load" #() {{ Φ }}.
   Proof.
-    wp_start as "[#Hint Hfupd]".
+    iIntros (Φ) "(#? & #Hint & Hau)".
+    wp_method_call. wp_call.
     iNamed "Hint".
     wp_auto.
+
     wp_apply (wp_Mutex__Lock with "[$Hlock]").
     iIntros "[Hlocked Hinv]". iNamed "Hinv".
     wp_auto.
-    iMod ("Hfupd" with "HP") as "[HQ HP]".
+
+    iApply fupd_wp.
+    iMod "Hau" as (x0) "[Hown Hclose]".
+    iDestruct (ghost_var_agree with "Hauth Hown") as %Heq; subst x0.
+    iMod ("Hclose" with "Hown") as "HΦ".
+    iModIntro.
+
     wp_alloc map_val as "Hmap".
     wp_auto.
-    wp_apply (wp_Mutex__Unlock with "[$Hlock $Hlocked HP val]").
+    wp_apply (wp_Mutex__Unlock with "[$Hlock $Hlocked Hauth val]").
     { iFrame. }
 
-    wp_finish.
+    iApply "HΦ".
   Qed.
 
-  Lemma wp_atomicPtr__store l (P: loc → iProp _) (Q: loc → iProp _) (y: loc) :
-    {{{ is_pkg_init hashmap ∗ is_atomic_ptr l P ∗
-          (∀ x, P x -∗ |={⊤}=> Q x ∗ P y) }}}
-      l @ (ptrT.id hashmap.atomicPtr.id) @ "store" #y
-    {{{ (x: loc), RET #(); Q x }}}.
+  Lemma wp_atomicPtr__store γ l (y: loc) :
+    ∀ Φ,
+    (is_pkg_init hashmap ∗ is_atomic_ptr γ l ∗
+    |={⊤,∅}=> ∃ x, own_ptr γ x ∗ (own_ptr γ y ={∅,⊤}=∗ Φ #())) -∗
+    WP l @ (ptrT.id hashmap.atomicPtr.id) @ "store" #y {{ Φ }}.
   Proof.
-    wp_start as "[#Hint Hfupd]".
+    iIntros (Φ) "(#? & #Hint & Hau)".
+    wp_method_call. wp_call.
     iNamed "Hint".
     wp_auto.
+
     wp_apply (wp_Mutex__Lock with "[$Hlock]").
     iIntros "[Hlocked Hinv]". iNamed "Hinv".
     wp_auto.
 
-    iMod ("Hfupd" with "HP") as "[HQ HP]".
+    iApply fupd_wp.
+    iMod "Hau" as (x0) "[Hown Hclose]".
+    iDestruct (ghost_var_agree with "Hauth Hown") as %Heq; subst x0.
+    iMod (ghost_var_update_2 y with "Hauth Hown") as "[Hauth Hown]".
+    { rewrite dfrac_op_own Qp.half_half //. }
+    iMod ("Hclose" with "Hown") as "HΦ".
+    iModIntro.
 
-    wp_apply (wp_Mutex__Unlock with "[$Hlock $Hlocked HP val]").
+    wp_apply (wp_Mutex__Unlock with "[$Hlock $Hlocked Hauth val]").
     { iFrame. }
 
-    wp_finish.
+    iApply "HΦ".
   Qed.
 
 End proof.
@@ -102,77 +130,71 @@ Import atomic_ptr.
 
 Section proof.
   Context `{hG: !heapGS Σ} `{!globalsGS Σ} {go_ctx: GoContext}.
+  Context `{!ghost_varG Σ loc}.
   Context `{!ghost_varG Σ (gmap w64 w64)}.
 
-  Definition ptr_rep (γ: gname) (P: gmap w64 w64 → iProp _) (mref: loc): iProp _ :=
-      ∃ (m: gmap w64 w64),
-      "#Hm_clean" ∷ own_map mref DfracDiscarded m ∗
-      "HP" ∷ P m ∗
-      "Hm_var" ∷ ghost_var γ (1/2) m
-      .
+  Let N := nroot .@ "hashmap".
 
-  Definition lock_inv (γ: gname): iProp _ :=
-    ∃ (m: gmap w64 w64),
-     "Hm_lock" ∷ ghost_var γ (1/2) m
-     .
-
-  (* Recall that the [P] argument is a representation invariant from the user of
-     the hashmap, which we need to maintain. Intuitively, [P m] should always hold
-     for some [m] that is the logically current state of the hashmap.
-
-    This hashmap implementation has an atomic pointer to a read-only copy of the
+  (* This hashmap implementation has an atomic pointer to a read-only copy of the
     map. Writes do a deep copy of the map to avoid disturbing reads.
 
-    The know from the state that the invariant for the hashmap consists of two
-    pieces: the representation predicate for the atomic pointer, and the lock
-    invariant. It turns out these two are enough (and we won't need a separate
-    invariant). Notice that we have the _caller_'s representation predicate [P]
-    for the actual map value, as well as the internal _hashmap_ predicate
-    [ptr_rep] for the map reference itself. We can guess that [ptr_rep] must
-    contain the caller's [P], since reads don't use the lock and yet still must
-    read the current value of the map.
+    In the TaDA style, we use ghost variables to track the logical state:
+    - γ_ptr: ghost variable tracking which map reference the atomic pointer holds
+    - γ_map: ghost variable tracking the logical value of the map
 
-    For writes, each operation gets the current value of the map, does a deep
-    copy (to allow modifications), and then stores the new map. We need a lock
-    to prevent a concurrent write from overlapping (think about how a write
-    could be lost if we didn't). So, the lock invariant captures that the
-    logical value of the map is frozen while the lock is held. We implement that
-    in Iris with a ghost variable whose value is the current map value - in
-    addition to maintaining [P m], we'll also have [ghost_var γ q m]. That ghost
-    variable will be half owned by the atomic pointer (since it needs to match
-    the physical state), and half owned by the _lock invariant_. This means upon
-    acquiring the lock the write operation knows the current value of the map
-    can no longer change, while still allowing reads.
+    The internal invariant [hashmap_inv] relates the pointer's current mref
+    (tracked by γ_ptr) to the actual map contents stored at that location.
+    Half of γ_map is owned by the lock invariant (so writes can freeze the logical
+    value), and half is given to the user via [own_hashmap].
    *)
 
-  Definition is_hashmap (l: loc) (P: gmap w64 w64 → iProp _): iProp _ :=
-    ∃ (ptr_l mu_l: loc) γ,
+  Definition own_hashmap γ (m: gmap w64 w64) :=
+    ghost_var γ (DfracOwn (1/2)) m.
+
+  #[global] Instance own_hashmap_timeless γ m : Timeless (own_hashmap γ m).
+  Proof. apply _. Qed.
+
+  Definition hashmap_inv γ γ_ptr : iProp _ :=
+    ∃ (mref: loc) (m: gmap w64 w64),
+    "Hptr" ∷ atomic_ptr.own_ptr γ_ptr mref ∗
+    "#Hm_clean" ∷ own_map mref DfracDiscarded m ∗
+    "Hm_var" ∷ ghost_var γ (DfracOwn (1/4)) m.
+
+  Definition lock_inv (γ_map: gname): iProp _ :=
+    ∃ (m: gmap w64 w64),
+     "Hm_lock" ∷ ghost_var γ_map (DfracOwn (1/4)) m
+  .
+
+  Definition is_hashmap γ γ_ptr (l: loc) : iProp _ :=
+    ∃ (ptr_l mu_l: loc),
     "#clean" ∷ l ↦s[hashmap.HashMap :: "clean"]□ ptr_l ∗
     "#mu" ∷ l ↦s[hashmap.HashMap :: "mu"]□ mu_l ∗
-    "#Hclean" ∷ is_atomic_ptr ptr_l (ptr_rep γ P) ∗
-    "#Hlock" ∷ is_Mutex mu_l (lock_inv γ)
-    .
+    "#Hclean" ∷ is_atomic_ptr γ_ptr ptr_l ∗
+    "#Hlock" ∷ is_Mutex mu_l (lock_inv γ) ∗
+    "#Hinv" ∷ inv N (hashmap_inv γ γ_ptr).
 
-  #[global] Instance is_hashmap_persistent l P : Persistent (is_hashmap l P) := _.
+  #[global] Instance is_hashmap_persistent γ γ_ptr l : Persistent (is_hashmap γ γ_ptr l) := _.
 
-  Lemma wp_NewHashMap (P: gmap w64 w64 → iProp _) :
-    {{{ is_pkg_init hashmap ∗ P ∅ }}}
+  Lemma wp_NewHashMap :
+    {{{ is_pkg_init hashmap }}}
       @! hashmap.NewHashMap #()
-    {{{ (l: loc), RET #l; is_hashmap l P }}}.
+    {{{ γ γ_ptr (l: loc), RET #l; is_hashmap γ γ_ptr l ∗ own_hashmap γ ∅ }}}.
   Proof.
-    wp_start as "HP".
+    wp_start as "_".
     wp_auto.
     wp_apply (wp_map_make (K:=w64) (V:=w64)) as "%mref Hm".
     { reflexivity. }
     iPersist "Hm".
-    iMod (ghost_var_alloc (∅: gmap w64 w64)) as (γ) "[Hm_var Hm_lock]".
-    wp_apply (wp_newAtomicPtr (ptr_rep γ P) with "[Hm_var $HP]").
-    { iFrame "∗#". }
-    iIntros (ptr_l) "Hptr".
+    iMod (ghost_var_alloc (∅: gmap w64 w64)) as (γ) "[[Hm_inv Hm_lock_inv] Hm_user]".
+    wp_apply (wp_newAtomicPtr mref).
+    iIntros (γ_ptr ptr_l) "[Hptr Hown_ptr]".
     wp_auto.
     wp_alloc mu_l as "Hmu".
     wp_auto.
-    iMod (init_Mutex (lock_inv γ) with "Hmu [$Hm_lock]") as "Hlock".
+    replace (1/2/2)%Qp with (1/4)%Qp by compute_done.
+    iMod (init_Mutex (lock_inv γ) with "Hmu [$Hm_lock_inv]") as "Hlock".
+    iMod (inv_alloc N _ (hashmap_inv γ γ_ptr) with "[Hown_ptr Hm_inv]") as "#Hinv".
+    { iModIntro. iFrame "∗#". }
     wp_alloc l as "Hmap".
     iApply struct_fields_split in "Hmap". iNamed "Hmap".
     cbn [hashmap.HashMap.clean' hashmap.HashMap.mu'].
@@ -218,30 +240,51 @@ Section proof.
   Definition map_get `{!IntoVal V} `{!IntoValTyped V t} (v: option V) : V * bool :=
     (default (default_val V) v, bool_decide (is_Some v)).
 
-  Lemma wp_HashMap__Load l (key: w64) (P: gmap w64 w64 → iProp _)
-    (Q: (w64 * bool) → iProp _) :
-  {{{ is_pkg_init hashmap ∗
-        is_hashmap l P ∗ (∀ m, P m ={⊤}=∗ Q (map_get (m !! key)) ∗ P m) }}}
-    l @ (ptrT.id hashmap.HashMap.id) @ "Load" #key
-  {{{ (v: w64) (ok: bool), RET (#v, #ok); Q (v, ok) }}}.
+  (* FIXME: eventually use upstream perennial instance *)
+  #[global] Instance own_map_timeless
+  `{!IntoVal K} `{!EqDecision K} `{!Countable K} `{!IntoVal V}
+    mptr dq (m: gmap K V)
+  `{!IntoValTyped K kt} `{!IntoValTyped V vt}
+    : Timeless (own_map mptr dq m).
+  Proof. rewrite own_map_unseal. apply _. Qed.
+
+  Lemma wp_HashMap__Load γ γ_ptr l (key: w64) :
+    ∀ (Φ: val → iProp Σ),
+    (is_pkg_init hashmap ∗
+    is_hashmap γ γ_ptr l ∗
+    |={⊤∖↑N,∅}=> ∃ m, own_hashmap γ m ∗ (own_hashmap γ m ={∅,⊤∖↑N}=∗ Φ (#(fst (map_get (m !! key))), #(snd (map_get (m !! key))))%V)) -∗
+    WP l @ (ptrT.id hashmap.HashMap.id) @ "Load" #key {{ Φ }}.
   Proof.
-    wp_start as "[#Hmap Hfupd]". iNamed "Hmap".
+    iIntros (Φ) "(#? & #Hmap & Hau)".
+    wp_method_call. wp_call.
+    iNamed "Hmap".
     wp_auto.
     wp_alloc clean_m_ptr as "Hnew_clean".
     wp_auto.
-    wp_apply (wp_atomicPtr__load _ _ (λ mref,
-      ∃ m, own_map mref DfracDiscarded m ∗
-      Q (map_get (m !! key))
-    )%I with "[$Hclean Hfupd]").
 
-    { iIntros (mref) "Hrep". iNamed "Hrep".
-      iMod ("Hfupd" with "HP") as "[HQ HP]".
-      iModIntro.
-      iFrame "#∗". }
+    wp_apply (wp_atomicPtr__load). iFrame "Hclean".
+    (* Now we prove the atomic update of the load. The linearization point of
+    loading this pointer is _also_ the linearization point for the hashmap
+    load, so we need to both open our invariant (to get temporary ownership of
+    the pointer) and fire the user's AU while we have a chance. *)
+    iInv "Hinv" as ">HI" "Hclose".
+    iMod "Hau" as (m) "[Hm Hau]".
+    iNamedSuffix "HI" "_inv".
+    iModIntro.
+    iFrame "Hptr_inv". iIntros "Hptr_inv".
+    (* this is the crucial information we learn from opening the invariant
+    (other than this, we open and close it as-is, since this operation is
+    read-only) *)
+    iDestruct (ghost_var_agree with "Hm_var_inv Hm") as %<-.
+    iMod ("Hau" with "Hm") as "HΦ".
 
-    iIntros (mref) "(%m & #Hclean_map & HQ)".
+    (* Close the hashmap invariant *)
+    iMod ("Hclose" with "[$Hptr_inv $Hm_var_inv]").
+    { iModIntro. iFrame "∗#". }
+
+    iModIntro.
     wp_auto.
-    wp_apply (wp_map_get with "[$Hclean_map]").
+    wp_apply (wp_map_get with "[$]").
     iIntros "_".
     wp_auto.
     wp_finish.
@@ -253,103 +296,153 @@ Section proof.
   abstract state due to the [ghost_var] premise, and it is exactly the map
   returned as physical state. We can also see the spec returns [own_map] with a
   fraction of [1] due to the deep copy here. *)
-  Lemma wp_HashMap__dirty (γ: gname) l (ptr_l: loc) (P: gmap w64 w64 → iProp _) (m: gmap w64 w64) :
+  Lemma wp_HashMap__dirty (γ γ_ptr: gname) l (ptr_l: loc) (m: gmap w64 w64) :
     {{{ is_pkg_init hashmap ∗
         "#clean" ∷ l ↦s[hashmap.HashMap :: "clean"]□ ptr_l ∗
-        "#Hclean" ∷ is_atomic_ptr ptr_l (ptr_rep γ P) ∗
-        "Hm_lock" ∷ ghost_var γ (1/2) m }}}
+        "#Hclean" ∷ is_atomic_ptr γ_ptr ptr_l ∗
+        "#Hinv" ∷ inv N (hashmap_inv γ γ_ptr) ∗
+        "Hm_lock" ∷ ghost_var γ (DfracOwn (1/4)) m }}}
       l @ (ptrT.id hashmap.HashMap.id) @ "dirty" #()
     {{{ (mref: loc), RET #mref;
       own_map (kt:=uint64T) mref (DfracOwn 1) m ∗
-      ghost_var γ (1/2) m }}}.
+      ghost_var γ (DfracOwn (1/4)) m }}}.
   Proof.
     wp_start as "Hpre". iNamed "Hpre".
     wp_auto.
     wp_alloc new_clean_ptr as "Hnew_clean".
     wp_auto.
-    wp_apply (wp_atomicPtr__load _ _ (λ mref,
-      (* the important part is that this [m] matches the one in the precondition, because of the ghost variable *)
-     own_map (kt:=uint64T) mref DfracDiscarded m ∗ ghost_var γ (1/2) m)%I
-     with "[$Hclean Hm_lock]").
-    { iIntros (mref) "Hrep". iNamed "Hrep".
-      iDestruct (ghost_var_agree with "Hm_lock Hm_var") as %<-.
-      iModIntro. iFrame "#∗". }
-      iIntros (mref) "(Hclean_m & Hm)".
-      wp_auto.
-      wp_apply (wp_mapClone with "[$Hclean_m]").
-      iIntros (mref') "Hdirty".
-      wp_auto.
-      wp_finish.
+
+    wp_apply (wp_atomicPtr__load). iFrame "Hclean".
+    (* Open hashmap invariant to get pointer ownership *)
+    iInv "Hinv" as ">HI" "Hclose_inv".
+    iApply fupd_mask_intro; [ set_solver | iIntros "Hmask" ].
+    iNamedSuffix "HI" "_inv".
+
+    (* Give pointer ownership to atomic_ptr *)
+    iFrame "Hptr_inv". iIntros "Hptr_inv".
+
+    (* Obtain that the map values agree *)
+    iMod "Hmask" as "_".
+    iDestruct (ghost_var_agree with "Hm_var_inv Hm_lock") as %<-.
+
+    (* Close the invariant *)
+    iMod ("Hclose_inv" with "[Hptr_inv Hm_var_inv]").
+    { iModIntro. iFrame "∗#". }
+
+    iModIntro.
+    wp_auto.
+    wp_apply (wp_mapClone with "[$]").
+    iIntros (mref') "Hdirty".
+    wp_auto.
+    wp_finish.
   Qed.
 
-  Lemma wp_HashMap__Store l (key: w64) (val: w64) (P: gmap w64 w64 → iProp _)
-    (Q: gmap w64 w64 → iProp _) :
-  {{{ is_pkg_init hashmap ∗
-      is_hashmap l P ∗
-      (∀ m, P m ={⊤}=∗ Q m ∗ P (map_insert key val m)) }}}
-    l @ (ptrT.id hashmap.HashMap.id) @ "Store" #key #val
-  {{{ m, RET #(); Q m }}}.
+  Lemma wp_HashMap__Store γ γ_ptr l (key: w64) (val: w64) :
+    ∀ Φ,
+    (is_pkg_init hashmap ∗
+    is_hashmap γ γ_ptr l ∗
+    |={⊤ ∖ ↑N,∅}=> ∃ m, own_hashmap γ m ∗
+        (own_hashmap γ (map_insert key val m) ={∅,⊤ ∖ ↑N}=∗ Φ #())) -∗
+    WP l @ (ptrT.id hashmap.HashMap.id) @ "Store" #key #val {{ Φ }}.
   Proof.
-    wp_start as "[#Hmap Hfupd]".
+    iIntros (Φ) "(#? & #Hmap & Hau)".
+    wp_method_call. wp_call.
     iNamed "Hmap".
     wp_auto.
-    wp_apply (wp_Mutex__Lock with "[$Hlock]"). iIntros "[Hlocked Hinv]".
-    iNamed "Hinv".
+    wp_apply (wp_Mutex__Lock with "[$Hlock]"). iIntros "[Hlocked Hlock_inv]".
+    iNamed "Hlock_inv".
     wp_auto.
-    wp_apply (wp_HashMap__dirty with "[$clean $Hclean $Hm_lock]").
+    wp_apply (wp_HashMap__dirty with "[$clean $Hclean $Hinv $Hm_lock]").
     iIntros (mref) "[Hdirty Hm_lock]".
     wp_auto.
     wp_apply (wp_map_insert with "Hdirty").
     iIntros "Hm".
     iPersist "Hm" as "Hm_new".
     wp_auto.
-    wp_apply (wp_atomicPtr__store _ _
-      (λ _, Q m ∗ ghost_var γ (1/2) (map_insert key val m))%I
-     with "[$Hclean Hfupd Hm_lock]").
-    { iIntros (mref') "Hrep". iNamed "Hrep".
-      iDestruct (ghost_var_agree with "Hm_lock Hm_var") as %<-.
-      iMod (ghost_var_update_halves (map_insert key val m) with "Hm_lock Hm_var") as "[Hm_lock Hm_var]".
-      iMod ("Hfupd" with "HP") as "[HQ HP]".
-      iModIntro.
-      iFrame "∗#". }
-    iIntros (_) "[HQ Hm_lock]".
+
+    wp_apply (wp_atomicPtr__store). iFrame "Hclean".
+    (* Open hashmap invariant *)
+    iInv "Hinv" as ">HI" "Hclose_inv".
+    iMod "Hau" as (m0) "[Hown Hclose_au]".
+    iNamedSuffix "HI" "_inv".
+    iModIntro.
+
+    (* Give old pointer ownership, get new pointer ownership *)
+    iFrame "Hptr_inv". iIntros "Hptr_inv".
+
+    (* Update ghost variables and execute user's AU *)
+    iDestruct (ghost_var_agree with "Hm_var_inv Hm_lock") as %<-.
+    iDestruct (ghost_var_agree with "Hm_var_inv Hown") as %<-.
+    iCombine "Hm_lock Hm_var_inv" as "Hm1".
+    rewrite Qp.quarter_quarter.
+    iMod (ghost_var_update_2 (<[key:=val]> m1) with "Hm1 Hown") as "[Hm1 Hown]".
+    { rewrite dfrac_op_own Qp.half_half //. }
+    iDestruct "Hm1" as "[Hm_lock Hm_var_inv]".
+    iMod ("Hclose_au" with "Hown") as "HΦ".
+    replace (1/2/2)%Qp with (1/4)%Qp by compute_done.
+
+    (* Close invariant with new map value *)
+    iMod ("Hclose_inv" with "[Hptr_inv Hm_var_inv]").
+    { iModIntro. iFrame "∗#". }
+
+    iModIntro.
     wp_auto.
     wp_apply (wp_Mutex__Unlock with "[$Hlock $Hlocked Hm_lock]").
     { iFrame. }
     wp_finish.
   Qed.
 
-  Lemma wp_HashMap__Delete l (key: w64) (P: gmap w64 w64 → iProp _)
-    (Q: gmap w64 w64 → iProp _) :
-  {{{ is_pkg_init hashmap ∗
-      is_hashmap l P ∗
-      (∀ m, P m ={⊤}=∗ Q m ∗ P (delete key m)) }}}
-    l @ (ptrT.id hashmap.HashMap.id) @ "Delete" #key
-  {{{ m, RET #(); Q m }}}.
+  Lemma wp_HashMap__Delete γ γ_ptr l (key: w64) :
+    ∀ Φ,
+    (is_pkg_init hashmap ∗
+    is_hashmap γ γ_ptr l ∗
+    |={⊤ ∖ ↑N,∅}=> ∃ m, own_hashmap γ m ∗
+        (own_hashmap γ (delete key m) ={∅,⊤ ∖ ↑N}=∗ Φ #())) -∗
+    WP l @ (ptrT.id hashmap.HashMap.id) @ "Delete" #key {{ Φ }}.
   Proof.
-    wp_start as "[#Hmap Hfupd]".
+    (* notice how this proof is nearly identical to that for Store: the way this
+    code works generally achieves atomicity for any critical section *)
+    iIntros (Φ) "(#? & #Hmap & Hau)".
+    wp_method_call. wp_call.
     iNamed "Hmap".
     wp_auto.
-    wp_apply (wp_Mutex__Lock with "[$Hlock]"). iIntros "[Hlocked Hinv]".
-    iNamed "Hinv".
+    wp_apply (wp_Mutex__Lock with "[$Hlock]"). iIntros "[Hlocked Hlock_inv]".
+    iNamed "Hlock_inv".
     wp_auto.
-    wp_apply (wp_HashMap__dirty with "[$clean $Hclean $Hm_lock]").
+    wp_apply (wp_HashMap__dirty with "[$clean $Hclean $Hinv $Hm_lock]").
     iIntros (mref) "[Hdirty Hm_lock]".
     wp_auto.
     wp_apply (wp_map_delete with "Hdirty").
     iIntros "Hm".
     iPersist "Hm" as "Hm_new".
     wp_auto.
-    wp_apply (wp_atomicPtr__store _ _
-      (λ _, Q m ∗ ghost_var γ (1/2) (delete key m))%I
-     with "[$Hclean Hfupd Hm_lock]").
-    { iIntros (mref') "Hrep". iNamed "Hrep".
-      iDestruct (ghost_var_agree with "Hm_lock Hm_var") as %<-.
-      iMod (ghost_var_update_halves (map_delete key m) with "Hm_lock Hm_var") as "[Hm_lock Hm_var]".
-      iMod ("Hfupd" with "HP") as "[HQ HP]".
-      iModIntro.
-      iFrame "∗#". }
-    iIntros (_) "[HQ Hm_lock]".
+
+    wp_apply (wp_atomicPtr__store). iFrame "Hclean".
+    (* Open hashmap invariant *)
+    iInv "Hinv" as ">HI" "Hclose_inv".
+    iMod "Hau" as (m0) "[Hown Hclose_au]".
+    iNamedSuffix "HI" "_inv".
+    iModIntro.
+
+    (* Give old pointer ownership, get new pointer ownership *)
+    iFrame "Hptr_inv". iIntros "Hptr_inv".
+
+    (* Update ghost variables and execute user's AU *)
+    iDestruct (ghost_var_agree with "Hm_var_inv Hm_lock") as %<-.
+    iDestruct (ghost_var_agree with "Hm_var_inv Hown") as %<-.
+    iCombine "Hm_lock Hm_var_inv" as "Hm1".
+    rewrite Qp.quarter_quarter.
+    iMod (ghost_var_update_2 (delete key m1) with "Hm1 Hown") as "[Hm1 Hown]".
+    { rewrite dfrac_op_own Qp.half_half //. }
+    iDestruct "Hm1" as "[Hm_lock Hm_var_inv]".
+    iMod ("Hclose_au" with "Hown") as "HΦ".
+    replace (1/2/2)%Qp with (1/4)%Qp by compute_done.
+
+    (* Close invariant with new map value *)
+    iMod ("Hclose_inv" with "[Hptr_inv Hm_var_inv]").
+    { iModIntro. iFrame "∗#". }
+
+    iModIntro.
     wp_auto.
     wp_apply (wp_Mutex__Unlock with "[$Hlock $Hlocked Hm_lock]").
     { iFrame. }
